append api

src/computational_monads/simulation_semantics/oracle_append.lean
@@ -5,34 +5,40 @@ import computational_monads.simulation_semantics.constructions.stateless_oracle
 open oracle_comp oracle_spec
 
 variables {spec spec' spec'' : oracle_spec} {A B C : Type}
+  (a : A) (oa : oracle_comp (spec' ++ spec'') A)
+  (ob : A → oracle_comp (spec' ++ spec'') B)
 
 section oracle_append
 
-def oracle_append (so : simulation_oracle spec' spec)
-  (so' : simulation_oracle spec'' spec) :
-  simulation_oracle (spec' ++ spec'') spec :=
+def oracle_append (so : simulation_oracle spec spec'')
+  (so' : simulation_oracle spec' spec'') :
+  simulation_oracle (spec ++ spec') spec'' :=
 { S := so.S × so'.S,
   default_state := (so.default_state, so'.default_state),
   o := λ i, match i with
-  | sum.inl i := λ ⟨t, s⟩, do { ⟨u, s'⟩ ← so.o i ⟨t, s.1⟩, return (u, s', s.2) }
-  | sum.inr i := λ ⟨t, s⟩, do { ⟨u, s'⟩ ← so'.o i ⟨t, s.2⟩, return (u, s.1, s') }
+  | sum.inl i := λ ⟨t, s⟩, do { ⟨u, s'⟩ ← so.o i ⟨t, s.1⟩, pure (u, s', s.2) }
+  | sum.inr i := λ ⟨t, s⟩, do { ⟨u, s'⟩ ← so'.o i ⟨t, s.2⟩, pure (u, s.1, s') }
   end }
 
 notation so `⟪++⟫` so' := oracle_append so so'
 
-variables (so : simulation_oracle spec' spec) (so' : simulation_oracle spec'' spec)
+variables (so : simulation_oracle spec spec'') (so' : simulation_oracle spec' spec'')
+  (i : spec.ι) (i' : spec'.ι) (t : spec.domain i) (t' : spec'.domain i')
+  (s : so.S × so'.S)
 
 @[simp]
-lemma default_state_oracle_append :
-  (so ⟪++⟫ so').default_state = (so.default_state, so'.default_state) := rfl
+lemma default_state_oracle_append : (so ⟪++⟫ so').default_state =
+  (so.default_state, so'.default_state) := rfl
+
+@[simp]
+lemma oracle_append_apply_inl : (so ⟪++⟫ so').o (sum.inl i) (t, s) =
+  so.o i (t, s.1) >>= λ ⟨u, s'⟩, pure (u, s', s.2) :=
+begin
+  simp [oracle_append],
+  sorry
+end
+
+-- @[simp]
+-- lemma simulate_oracle_append_pure : simulate (so ⟪++⟫ so') (pure a) s ≃ₚ
 
 end oracle_append
-
-section simulate_sides
-
-def simulate_right {spec spec' : oracle_spec}
-  (so : simulation_oracle spec' spec) :
-  simulation_oracle (spec ++ spec') spec :=
-identity_oracle spec ⟪++⟫ so
-
-end simulate_sides
